formal/fstar/ocaml-output/JSONLD_FromRdf.ml
@@ -1,0 +1,710 @@
+open Prims
+type from_rdf_options =
+  {
+  use_native_types: Prims.bool ;
+  use_rdf_type: Prims.bool ;
+  rdf_direction: Prims.string FStar_Pervasives_Native.option }
+let __proj__Mkfrom_rdf_options__item__use_native_types
+  (projectee : from_rdf_options) : Prims.bool=
+  match projectee with
+  | { use_native_types; use_rdf_type; rdf_direction;_} -> use_native_types
+let __proj__Mkfrom_rdf_options__item__use_rdf_type
+  (projectee : from_rdf_options) : Prims.bool=
+  match projectee with
+  | { use_native_types; use_rdf_type; rdf_direction;_} -> use_rdf_type
+let __proj__Mkfrom_rdf_options__item__rdf_direction
+  (projectee : from_rdf_options) :
+  Prims.string FStar_Pervasives_Native.option=
+  match projectee with
+  | { use_native_types; use_rdf_type; rdf_direction;_} -> rdf_direction
+let default_options : from_rdf_options=
+  {
+    use_native_types = false;
+    use_rdf_type = false;
+    rdf_direction = FStar_Pervasives_Native.None
+  }
+let rdf_type_iri : Prims.string=
+  "http://www.w3.org/1999/02/22-rdf-syntax-ns#type"
+let rdf_first_iri : Prims.string=
+  "http://www.w3.org/1999/02/22-rdf-syntax-ns#first"
+let rdf_rest_iri : Prims.string=
+  "http://www.w3.org/1999/02/22-rdf-syntax-ns#rest"
+let rdf_nil_iri : Prims.string=
+  "http://www.w3.org/1999/02/22-rdf-syntax-ns#nil"
+let rdf_json_iri : Prims.string=
+  "http://www.w3.org/1999/02/22-rdf-syntax-ns#JSON"
+let rdf_list_iri : Prims.string=
+  "http://www.w3.org/1999/02/22-rdf-syntax-ns#List"
+let rdf_value_iri : Prims.string=
+  "http://www.w3.org/1999/02/22-rdf-syntax-ns#value"
+let rdf_direction_iri : Prims.string=
+  "http://www.w3.org/1999/02/22-rdf-syntax-ns#direction"
+let rdf_language_iri : Prims.string=
+  "http://www.w3.org/1999/02/22-rdf-syntax-ns#language"
+let i18n_prefix : Prims.string= "https://www.w3.org/ns/i18n#"
+let sxsd_string : Prims.string= RDF_Term.xsd_string
+let sxsd_integer : Prims.string= RDF_Term.xsd_integer
+let sxsd_double : Prims.string= RDF_Term.xsd_double
+let sxsd_boolean : Prims.string= RDF_Term.xsd_boolean
+let strcat (a : Prims.string) (b : Prims.string) : Prims.string=
+  FStar_String.concat "" [a; b]
+type ov =
+  | OV_Ref of Prims.string 
+  | OV_Val of Parser_JSON.json_val 
+  | OV_List of ov Prims.list 
+let uu___is_OV_Ref (projectee : ov) : Prims.bool=
+  match projectee with | OV_Ref _0 -> true | uu___ -> false
+let __proj__OV_Ref__item___0 (projectee : ov) : Prims.string=
+  match projectee with | OV_Ref _0 -> _0
+let uu___is_OV_Val (projectee : ov) : Prims.bool=
+  match projectee with | OV_Val _0 -> true | uu___ -> false
+let __proj__OV_Val__item___0 (projectee : ov) : Parser_JSON.json_val=
+  match projectee with | OV_Val _0 -> _0
+let uu___is_OV_List (projectee : ov) : Prims.bool=
+  match projectee with | OV_List _0 -> true | uu___ -> false
+let __proj__OV_List__item___0 (projectee : ov) : ov Prims.list=
+  match projectee with | OV_List _0 -> _0
+type fr_node =
+  {
+  n_id: Prims.string ;
+  n_blank: Prims.bool ;
+  n_types: Prims.string Prims.list ;
+  n_props: (Prims.string * ov Prims.list) Prims.list }
+let __proj__Mkfr_node__item__n_id (projectee : fr_node) : Prims.string=
+  match projectee with | { n_id; n_blank; n_types; n_props;_} -> n_id
+let __proj__Mkfr_node__item__n_blank (projectee : fr_node) : Prims.bool=
+  match projectee with | { n_id; n_blank; n_types; n_props;_} -> n_blank
+let __proj__Mkfr_node__item__n_types (projectee : fr_node) :
+  Prims.string Prims.list=
+  match projectee with | { n_id; n_blank; n_types; n_props;_} -> n_types
+let __proj__Mkfr_node__item__n_props (projectee : fr_node) :
+  (Prims.string * ov Prims.list) Prims.list=
+  match projectee with | { n_id; n_blank; n_types; n_props;_} -> n_props
+type named_nm =
+  {
+  gn_name: Prims.string ;
+  gn_blank: Prims.bool ;
+  gn_map: fr_node Prims.list }
+let __proj__Mknamed_nm__item__gn_name (projectee : named_nm) : Prims.string=
+  match projectee with | { gn_name; gn_blank; gn_map;_} -> gn_name
+let __proj__Mknamed_nm__item__gn_blank (projectee : named_nm) : Prims.bool=
+  match projectee with | { gn_name; gn_blank; gn_map;_} -> gn_blank
+let __proj__Mknamed_nm__item__gn_map (projectee : named_nm) :
+  fr_node Prims.list=
+  match projectee with | { gn_name; gn_blank; gn_map;_} -> gn_map
+let subj_id (s : RDF_Term.subject) : Prims.string=
+  match s with | RDF_Term.S_IRI i -> i | RDF_Term.S_BNode b -> strcat "_:" b
+let subj_is_blank (s : RDF_Term.subject) : Prims.bool=
+  RDF_Term.uu___is_S_BNode s
+let term_node_id (o : RDF_Term.rdf_term) :
+  (Prims.string * Prims.bool) FStar_Pervasives_Native.option=
+  match o with
+  | RDF_Term.T_IRI i -> FStar_Pervasives_Native.Some (i, false)
+  | RDF_Term.T_BNode b ->
+      FStar_Pervasives_Native.Some ((strcat "_:" b), true)
+  | RDF_Term.T_Literal uu___ -> FStar_Pervasives_Native.None
+let starts_with_us (s : Prims.string) : Prims.bool=
+  (((Parser_FastString.fs_byte_length s) >= (Prims.of_int (2))) &&
+     ((Parser_FastString.fs_byte_at s Prims.int_zero) = (Prims.of_int (0x5F))))
+    &&
+    ((Parser_FastString.fs_byte_at s Prims.int_one) = (Prims.of_int (0x3A)))
+let rec find_node (nm : fr_node Prims.list) (id : Prims.string) :
+  fr_node FStar_Pervasives_Native.option=
+  match nm with
+  | [] -> FStar_Pervasives_Native.None
+  | n::tl ->
+      if n.n_id = id then FStar_Pervasives_Native.Some n else find_node tl id
+let node_exists (nm : fr_node Prims.list) (id : Prims.string) : Prims.bool=
+  FStar_Pervasives_Native.uu___is_Some (find_node nm id)
+let ensure_node (nm : fr_node Prims.list) (id : Prims.string)
+  (blank : Prims.bool) : fr_node Prims.list=
+  if node_exists nm id
+  then nm
+  else
+    FStar_List_Tot_Base.op_At nm
+      [{ n_id = id; n_blank = blank; n_types = []; n_props = [] }]
+let rec snoc_unique : 'a . 'a Prims.list -> 'a -> 'a Prims.list =
+  fun xs x ->
+    match xs with
+    | [] -> [x]
+    | h::tl -> if h = x then xs else h :: (snoc_unique tl x)
+let rec find_prop (props : (Prims.string * ov Prims.list) Prims.list)
+  (p : Prims.string) : ov Prims.list FStar_Pervasives_Native.option=
+  match props with
+  | [] -> FStar_Pervasives_Native.None
+  | (k, vals)::tl ->
+      if k = p then FStar_Pervasives_Native.Some vals else find_prop tl p
+let node_prop_single (n : fr_node) (p : Prims.string) :
+  ov FStar_Pervasives_Native.option=
+  match find_prop n.n_props p with
+  | FStar_Pervasives_Native.Some (v::[]) -> FStar_Pervasives_Native.Some v
+  | uu___ -> FStar_Pervasives_Native.None
+let rec prop_add (props : (Prims.string * ov Prims.list) Prims.list)
+  (p : Prims.string) (v : ov) : (Prims.string * ov Prims.list) Prims.list=
+  match props with
+  | [] -> [(p, [v])]
+  | (k, vals)::tl ->
+      if k = p
+      then (k, (snoc_unique vals v)) :: tl
+      else (k, vals) :: (prop_add tl p v)
+let node_update_prop (nm : fr_node Prims.list) (id : Prims.string)
+  (p : Prims.string) (v : ov) : fr_node Prims.list=
+  FStar_List_Tot_Base.map
+    (fun n ->
+       if n.n_id = id
+       then
+         {
+           n_id = (n.n_id);
+           n_blank = (n.n_blank);
+           n_types = (n.n_types);
+           n_props = (prop_add n.n_props p v)
+         }
+       else n) nm
+let node_update_type (nm : fr_node Prims.list) (id : Prims.string)
+  (t : Prims.string) : fr_node Prims.list=
+  FStar_List_Tot_Base.map
+    (fun n ->
+       if n.n_id = id
+       then
+         {
+           n_id = (n.n_id);
+           n_blank = (n.n_blank);
+           n_types = (snoc_unique n.n_types t);
+           n_props = (n.n_props)
+         }
+       else n) nm
+let is_dec_digit (c : Prims.nat) : Prims.bool=
+  (c >= (Prims.of_int (0x30))) && (c <= (Prims.of_int (0x39)))
+let rec all_dec_digits (s : Prims.string) (pos : Prims.nat)
+  (fuel : Prims.nat) : Prims.bool=
+  if fuel = Prims.int_zero
+  then true
+  else
+    if pos >= (Parser_FastString.fs_byte_length s)
+    then true
+    else
+      if is_dec_digit (Parser_FastString.fs_byte_at s pos)
+      then all_dec_digits s (pos + Prims.int_one) (fuel - Prims.int_one)
+      else false
+let is_int_lexeme (s : Prims.string) : Prims.bool=
+  let n = Parser_FastString.fs_byte_length s in
+  if n = Prims.int_zero
+  then false
+  else
+    (let first = Parser_FastString.fs_byte_at s Prims.int_zero in
+     let start =
+       if (first = (Prims.of_int (0x2B))) || (first = (Prims.of_int (0x2D)))
+       then Prims.int_one
+       else Prims.int_zero in
+     (start < n) && (all_dec_digits s start ((n - start) + Prims.int_one)))
+let rec find_exp_char (s : Prims.string) (pos : Prims.nat) (fuel : Prims.nat)
+  : Prims.int=
+  if (fuel = Prims.int_zero) || (pos >= (Parser_FastString.fs_byte_length s))
+  then (Prims.of_int (-1))
+  else
+    (let c = Parser_FastString.fs_byte_at s pos in
+     if (c = (Prims.of_int (0x65))) || (c = (Prims.of_int (0x45)))
+     then pos
+     else find_exp_char s (pos + Prims.int_one) (fuel - Prims.int_one))
+let rec count_digits_from (s : Prims.string) (pos : Prims.nat)
+  (fuel : Prims.nat) : Prims.nat=
+  if (fuel = Prims.int_zero) || (pos >= (Parser_FastString.fs_byte_length s))
+  then Prims.int_zero
+  else
+    (let c = Parser_FastString.fs_byte_at s pos in
+     if is_dec_digit c
+     then
+       Prims.int_one +
+         (count_digits_from s (pos + Prims.int_one) (fuel - Prims.int_one))
+     else count_digits_from s (pos + Prims.int_one) (fuel - Prims.int_one))
+let is_finite_double (s : Prims.string) : Prims.bool=
+  match Parser_JSON.parse_json s with
+  | FStar_Pervasives_Native.Some (Parser_JSON.JNumber uu___) ->
+      let n = Parser_FastString.fs_byte_length s in
+      let ei = find_exp_char s Prims.int_zero (n + Prims.int_one) in
+      if ei < Prims.int_zero
+      then true
+      else
+        (count_digits_from s (ei + Prims.int_one) (n + Prims.int_one)) <=
+          (Prims.of_int (3))
+  | uu___ -> false
+let native_value (lex : Prims.string) (dt : Prims.string) : ov=
+  if dt = sxsd_boolean
+  then
+    (if (lex = "true") || (lex = "1")
+     then OV_Val (Parser_JSON.JObject [("@value", (Parser_JSON.JBool true))])
+     else
+       if (lex = "false") || (lex = "0")
+       then
+         OV_Val (Parser_JSON.JObject [("@value", (Parser_JSON.JBool false))])
+       else
+         OV_Val
+           (Parser_JSON.JObject
+              [("@value", (Parser_JSON.JString lex));
+              ("@type", (Parser_JSON.JString dt))]))
+  else
+    if dt = sxsd_integer
+    then
+      (if is_int_lexeme lex
+       then
+         OV_Val (Parser_JSON.JObject [("@value", (Parser_JSON.JNumber lex))])
+       else
+         OV_Val
+           (Parser_JSON.JObject
+              [("@value", (Parser_JSON.JString lex));
+              ("@type", (Parser_JSON.JString dt))]))
+    else
+      if dt = sxsd_double
+      then
+        (if is_finite_double lex
+         then
+           OV_Val
+             (Parser_JSON.JObject [("@value", (Parser_JSON.JNumber lex))])
+         else
+           OV_Val
+             (Parser_JSON.JObject
+                [("@value", (Parser_JSON.JString lex));
+                ("@type", (Parser_JSON.JString dt))]))
+      else
+        OV_Val
+          (Parser_JSON.JObject
+             [("@value", (Parser_JSON.JString lex));
+             ("@type", (Parser_JSON.JString dt))])
+let str_has_prefix (s : Prims.string) (pfx : Prims.string) : Prims.bool=
+  let ls = Parser_FastString.fs_byte_length s in
+  let lp = Parser_FastString.fs_byte_length pfx in
+  (ls >= lp) && ((Parser_FastString.fs_byte_sub s Prims.int_zero lp) = pfx)
+let rec last_us_pos (s : Prims.string) (pos : Prims.nat) (best : Prims.nat)
+  (fuel : Prims.nat) : Prims.nat=
+  if fuel = Prims.int_zero
+  then best
+  else
+    if pos >= (Parser_FastString.fs_byte_length s)
+    then best
+    else
+      last_us_pos s (pos + Prims.int_one)
+        (if (Parser_FastString.fs_byte_at s pos) = (Prims.of_int (0x5F))
+         then pos
+         else best) (fuel - Prims.int_one)
+let i18n_value_object (lex : Prims.string) (dt : Prims.string) : ov=
+  let lp = Parser_FastString.fs_byte_length i18n_prefix in
+  let dl = Parser_FastString.fs_byte_length dt in
+  let frag =
+    Parser_FastString.fs_byte_sub dt lp
+      (if dl >= lp then dl - lp else Prims.int_zero) in
+  let flen = Parser_FastString.fs_byte_length frag in
+  let up = last_us_pos frag Prims.int_zero flen (flen + Prims.int_one) in
+  let lang =
+    if up >= flen
+    then ""
+    else Parser_FastString.fs_byte_sub frag Prims.int_zero up in
+  let dir =
+    if up >= flen
+    then frag
+    else
+      Parser_FastString.fs_byte_sub frag (up + Prims.int_one)
+        (if flen > (up + Prims.int_one)
+         then (flen - up) - Prims.int_one
+         else Prims.int_zero) in
+  let base = [("@value", (Parser_JSON.JString lex))] in
+  let with_lang =
+    if (Parser_FastString.fs_byte_length lang) > Prims.int_zero
+    then
+      FStar_List_Tot_Base.op_At base
+        [("@language", (Parser_JSON.JString lang))]
+    else base in
+  OV_Val
+    (Parser_JSON.JObject
+       (FStar_List_Tot_Base.op_At with_lang
+          [("@direction", (Parser_JSON.JString dir))]))
+let rdf_to_object (opts : from_rdf_options) (o : RDF_Term.rdf_term) :
+  ov FStar_Pervasives_Native.option=
+  match o with
+  | RDF_Term.T_IRI i -> FStar_Pervasives_Native.Some (OV_Ref i)
+  | RDF_Term.T_BNode b ->
+      FStar_Pervasives_Native.Some (OV_Ref (strcat "_:" b))
+  | RDF_Term.T_Literal l ->
+      let lex = l.RDF_Term.lexical_form in
+      let dt = l.RDF_Term.datatype in
+      (match l.RDF_Term.lang_tag with
+       | FStar_Pervasives_Native.Some tag ->
+           FStar_Pervasives_Native.Some
+             (OV_Val
+                (Parser_JSON.JObject
+                   [("@value", (Parser_JSON.JString lex));
+                   ("@language", (Parser_JSON.JString tag))]))
+       | FStar_Pervasives_Native.None ->
+           if
+             (opts.rdf_direction =
+                (FStar_Pervasives_Native.Some "i18n-datatype"))
+               && (str_has_prefix dt i18n_prefix)
+           then FStar_Pervasives_Native.Some (i18n_value_object lex dt)
+           else
+             if dt = rdf_json_iri
+             then
+               (match Parser_JSON.parse_json lex with
+                | FStar_Pervasives_Native.Some j ->
+                    FStar_Pervasives_Native.Some
+                      (OV_Val
+                         (Parser_JSON.JObject
+                            [("@value", j);
+                            ("@type", (Parser_JSON.JString "@json"))]))
+                | FStar_Pervasives_Native.None ->
+                    FStar_Pervasives_Native.None)
+             else
+               if dt = sxsd_string
+               then
+                 FStar_Pervasives_Native.Some
+                   (OV_Val
+                      (Parser_JSON.JObject
+                         [("@value", (Parser_JSON.JString lex))]))
+               else
+                 if opts.use_native_types
+                 then FStar_Pervasives_Native.Some (native_value lex dt)
+                 else
+                   FStar_Pervasives_Native.Some
+                     (OV_Val
+                        (Parser_JSON.JObject
+                           [("@value", (Parser_JSON.JString lex));
+                           ("@type", (Parser_JSON.JString dt))])))
+let process_triple (opts : from_rdf_options) (nm : fr_node Prims.list)
+  (t : RDF_Triple.triple) :
+  fr_node Prims.list FStar_Pervasives_Native.option=
+  let s_id = subj_id t.RDF_Triple.s in
+  let s_blank = subj_is_blank t.RDF_Triple.s in
+  let nm1 = ensure_node nm s_id s_blank in
+  let nm2 =
+    match term_node_id t.RDF_Triple.o with
+    | FStar_Pervasives_Native.Some (oid, ob) -> ensure_node nm1 oid ob
+    | FStar_Pervasives_Native.None -> nm1 in
+  let p = t.RDF_Triple.p in
+  let obj_is_node =
+    (RDF_Term.uu___is_T_IRI t.RDF_Triple.o) ||
+      (RDF_Term.uu___is_T_BNode t.RDF_Triple.o) in
+  if
+    ((p = rdf_type_iri) && (Prims.op_Negation opts.use_rdf_type)) &&
+      obj_is_node
+  then
+    match term_node_id t.RDF_Triple.o with
+    | FStar_Pervasives_Native.Some (oid, uu___) ->
+        FStar_Pervasives_Native.Some (node_update_type nm2 s_id oid)
+    | FStar_Pervasives_Native.None -> FStar_Pervasives_Native.Some nm2
+  else
+    (match rdf_to_object opts t.RDF_Triple.o with
+     | FStar_Pervasives_Native.None -> FStar_Pervasives_Native.None
+     | FStar_Pervasives_Native.Some v ->
+         FStar_Pervasives_Native.Some (node_update_prop nm2 s_id p v))
+let rec build_nodemap (opts : from_rdf_options) (nm : fr_node Prims.list)
+  (ts : RDF_Triple.triple Prims.list) :
+  fr_node Prims.list FStar_Pervasives_Native.option=
+  match ts with
+  | [] -> FStar_Pervasives_Native.Some nm
+  | t::tl ->
+      (match process_triple opts nm t with
+       | FStar_Pervasives_Native.None -> FStar_Pervasives_Native.None
+       | FStar_Pervasives_Native.Some nm' -> build_nodemap opts nm' tl)
+let rec build_named (opts : from_rdf_options)
+  (ngs : RDF_Graph.named_graph Prims.list) :
+  named_nm Prims.list FStar_Pervasives_Native.option=
+  match ngs with
+  | [] -> FStar_Pervasives_Native.Some []
+  | ng::tl ->
+      (match build_nodemap opts [] ng.RDF_Graph.ng_graph with
+       | FStar_Pervasives_Native.None -> FStar_Pervasives_Native.None
+       | FStar_Pervasives_Native.Some m ->
+           (match build_named opts tl with
+            | FStar_Pervasives_Native.None -> FStar_Pervasives_Native.None
+            | FStar_Pervasives_Native.Some others ->
+                FStar_Pervasives_Native.Some
+                  ({
+                     gn_name = (ng.RDF_Graph.ng_name);
+                     gn_blank = (starts_with_us ng.RDF_Graph.ng_name);
+                     gn_map = m
+                   }
+                  :: others)))
+let rec add_graph_names (nm : fr_node Prims.list)
+  (named : named_nm Prims.list) : fr_node Prims.list=
+  match named with
+  | [] -> nm
+  | g::tl -> add_graph_names (ensure_node nm g.gn_name g.gn_blank) tl
+let rec is_graph_name (named : named_nm Prims.list) (id : Prims.string) :
+  Prims.bool=
+  match named with
+  | [] -> false
+  | g::tl -> if g.gn_name = id then true else is_graph_name tl id
+let rec lookup_graph_map (named : named_nm Prims.list) (id : Prims.string) :
+  fr_node Prims.list FStar_Pervasives_Native.option=
+  match named with
+  | [] -> FStar_Pervasives_Native.None
+  | g::tl ->
+      if g.gn_name = id
+      then FStar_Pervasives_Native.Some (g.gn_map)
+      else lookup_graph_map tl id
+let rec ovs_refids (vs : ov Prims.list) : Prims.string Prims.list=
+  match vs with
+  | [] -> []
+  | (OV_Ref x)::tl -> x :: (ovs_refids tl)
+  | uu___::tl -> ovs_refids tl
+let rec props_refids (props : (Prims.string * ov Prims.list) Prims.list) :
+  Prims.string Prims.list=
+  match props with
+  | [] -> []
+  | (uu___, vals)::tl ->
+      FStar_List_Tot_Base.op_At (ovs_refids vals) (props_refids tl)
+let rec nodes_refids (nm : fr_node Prims.list) : Prims.string Prims.list=
+  match nm with
+  | [] -> []
+  | n::tl ->
+      FStar_List_Tot_Base.op_At (props_refids n.n_props) (nodes_refids tl)
+let rec maps_refids (maps : fr_node Prims.list Prims.list) :
+  Prims.string Prims.list=
+  match maps with
+  | [] -> []
+  | m::tl -> FStar_List_Tot_Base.op_At (nodes_refids m) (maps_refids tl)
+let count_occ (xs : Prims.string Prims.list) (x : Prims.string) : Prims.nat=
+  FStar_List_Tot_Base.length (FStar_List_Tot_Base.filter (fun y -> y = x) xs)
+let referenced_once (refids : Prims.string Prims.list) (id : Prims.string) :
+  Prims.bool= (count_occ refids id) = Prims.int_one
+let rec obj_lookup
+  (fields : (Prims.string * Parser_JSON.json_val) Prims.list)
+  (k : Prims.string) : Parser_JSON.json_val FStar_Pervasives_Native.option=
+  match fields with
+  | [] -> FStar_Pervasives_Native.None
+  | (k2, v)::tl ->
+      if k2 = k then FStar_Pervasives_Native.Some v else obj_lookup tl k
+let cl_field (n : fr_node) (p : Prims.string) :
+  Parser_JSON.json_val FStar_Pervasives_Native.option=
+  match node_prop_single n p with
+  | FStar_Pervasives_Native.Some (OV_Val (Parser_JSON.JObject fields)) ->
+      obj_lookup fields "@value"
+  | uu___ -> FStar_Pervasives_Native.None
+let is_cl_shape (n : fr_node) : Prims.bool=
+  (n.n_blank &&
+     (FStar_Pervasives_Native.uu___is_Some (node_prop_single n rdf_value_iri)))
+    &&
+    (FStar_Pervasives_Native.uu___is_Some
+       (node_prop_single n rdf_direction_iri))
+let cl_value_object (n : fr_node) :
+  Parser_JSON.json_val FStar_Pervasives_Native.option=
+  match ((cl_field n rdf_value_iri), (cl_field n rdf_direction_iri)) with
+  | (FStar_Pervasives_Native.Some v, FStar_Pervasives_Native.Some d) ->
+      let lang = cl_field n rdf_language_iri in
+      FStar_Pervasives_Native.Some
+        (Parser_JSON.JObject
+           (FStar_List_Tot_Base.op_At [("@value", v)]
+              (FStar_List_Tot_Base.op_At
+                 (match lang with
+                  | FStar_Pervasives_Native.Some l -> [("@language", l)]
+                  | FStar_Pervasives_Native.None -> []) [("@direction", d)])))
+  | (uu___, uu___1) -> FStar_Pervasives_Native.None
+let is_cl_collapsible (g : fr_node Prims.list)
+  (refids : Prims.string Prims.list) (id : Prims.string) : Prims.bool=
+  match find_node g id with
+  | FStar_Pervasives_Native.None -> false
+  | FStar_Pervasives_Native.Some n ->
+      (is_cl_shape n) && (referenced_once refids id)
+let is_list_shape (n : fr_node) : Prims.bool=
+  (((n.n_blank && ((n.n_types = []) || (n.n_types = [rdf_list_iri]))) &&
+      ((FStar_List_Tot_Base.length n.n_props) = (Prims.of_int (2))))
+     &&
+     (FStar_Pervasives_Native.uu___is_Some (node_prop_single n rdf_first_iri)))
+    &&
+    (FStar_Pervasives_Native.uu___is_Some (node_prop_single n rdf_rest_iri))
+let rec is_collapsible (g : fr_node Prims.list)
+  (refids : Prims.string Prims.list) (id : Prims.string) (fuel : Prims.nat) :
+  Prims.bool=
+  if fuel = Prims.int_zero
+  then false
+  else
+    (match find_node g id with
+     | FStar_Pervasives_Native.None -> false
+     | FStar_Pervasives_Native.Some n ->
+         if Prims.op_Negation (is_list_shape n)
+         then false
+         else
+           if Prims.op_Negation (referenced_once refids id)
+           then false
+           else
+             (match node_prop_single n rdf_rest_iri with
+              | FStar_Pervasives_Native.Some (OV_Ref rt) ->
+                  if rt = rdf_nil_iri
+                  then true
+                  else is_collapsible g refids rt (fuel - Prims.int_one)
+              | uu___3 -> false))
+let rec list_from (g : fr_node Prims.list) (refids : Prims.string Prims.list)
+  (cl_mode : Prims.bool) (id : Prims.string) (fuel : Prims.nat) :
+  ov Prims.list=
+  if fuel = Prims.int_zero
+  then []
+  else
+    (match find_node g id with
+     | FStar_Pervasives_Native.None -> []
+     | FStar_Pervasives_Native.Some n ->
+         (match ((node_prop_single n rdf_first_iri),
+                  (node_prop_single n rdf_rest_iri))
+          with
+          | (FStar_Pervasives_Native.Some fv, FStar_Pervasives_Native.Some
+             (OV_Ref rt)) ->
+              let elem = resolve g refids cl_mode fv (fuel - Prims.int_one) in
+              if rt = rdf_nil_iri
+              then [elem]
+              else elem ::
+                (list_from g refids cl_mode rt (fuel - Prims.int_one))
+          | (uu___1, uu___2) -> []))
+and resolve (g : fr_node Prims.list) (refids : Prims.string Prims.list)
+  (cl_mode : Prims.bool) (v : ov) (fuel : Prims.nat) : ov=
+  if fuel = Prims.int_zero
+  then v
+  else
+    (match v with
+     | OV_Ref x ->
+         if x = rdf_nil_iri
+         then OV_List []
+         else
+           if is_collapsible g refids x fuel
+           then OV_List (list_from g refids cl_mode x (fuel - Prims.int_one))
+           else
+             if cl_mode && (is_cl_collapsible g refids x)
+             then
+               (match find_node g x with
+                | FStar_Pervasives_Native.Some n ->
+                    (match cl_value_object n with
+                     | FStar_Pervasives_Native.Some j -> OV_Val j
+                     | FStar_Pervasives_Native.None -> OV_Ref x)
+                | FStar_Pervasives_Native.None -> OV_Ref x)
+             else OV_Ref x
+     | OV_Val j -> OV_Val j
+     | OV_List l -> OV_List l)
+let rewrite_node (g : fr_node Prims.list) (refids : Prims.string Prims.list)
+  (cl_mode : Prims.bool) (fuel : Prims.nat) (n : fr_node) : fr_node=
+  {
+    n_id = (n.n_id);
+    n_blank = (n.n_blank);
+    n_types = (n.n_types);
+    n_props =
+      (FStar_List_Tot_Base.map
+         (fun pv ->
+            let uu___ = pv in
+            match uu___ with
+            | (p, vals) ->
+                (p,
+                  (FStar_List_Tot_Base.map
+                     (fun v -> resolve g refids cl_mode v fuel) vals)))
+         n.n_props)
+  }
+let rec ov_to_json (v : ov) : Parser_JSON.json_val=
+  match v with
+  | OV_Ref id -> Parser_JSON.JObject [("@id", (Parser_JSON.JString id))]
+  | OV_Val j -> j
+  | OV_List l ->
+      Parser_JSON.JObject
+        [("@list", (Parser_JSON.JArray (ov_list_to_json l)))]
+and ov_list_to_json (l : ov Prims.list) : Parser_JSON.json_val Prims.list=
+  match l with | [] -> [] | v::tl -> (ov_to_json v) :: (ov_list_to_json tl)
+let types_field (types : Prims.string Prims.list) :
+  (Prims.string * Parser_JSON.json_val) Prims.list=
+  if Prims.uu___is_Cons types
+  then
+    [("@type",
+       (Parser_JSON.JArray
+          (FStar_List_Tot_Base.map (fun t -> Parser_JSON.JString t) types)))]
+  else []
+let graph_field
+  (gj : Parser_JSON.json_val Prims.list FStar_Pervasives_Native.option) :
+  (Prims.string * Parser_JSON.json_val) Prims.list=
+  match gj with
+  | FStar_Pervasives_Native.Some gs -> [("@graph", (Parser_JSON.JArray gs))]
+  | FStar_Pervasives_Native.None -> []
+let props_fields (props : (Prims.string * ov Prims.list) Prims.list) :
+  (Prims.string * Parser_JSON.json_val) Prims.list=
+  FStar_List_Tot_Base.map
+    (fun pv ->
+       let uu___ = pv in
+       match uu___ with
+       | (p, vals) ->
+           (p,
+             (Parser_JSON.JArray (FStar_List_Tot_Base.map ov_to_json vals))))
+    props
+let node_to_json (n : fr_node)
+  (gj : Parser_JSON.json_val Prims.list FStar_Pervasives_Native.option) :
+  Parser_JSON.json_val=
+  Parser_JSON.JObject
+    (FStar_List_Tot_Base.op_At [("@id", (Parser_JSON.JString (n.n_id)))]
+       (FStar_List_Tot_Base.op_At (types_field n.n_types)
+          (FStar_List_Tot_Base.op_At (graph_field gj)
+             (props_fields n.n_props))))
+let rec insert_sorted_node (n : fr_node) (xs : fr_node Prims.list) :
+  fr_node Prims.list=
+  match xs with
+  | [] -> [n]
+  | h::tl ->
+      if RDF_Graph_Executable.string_lt n.n_id h.n_id
+      then n :: xs
+      else h :: (insert_sorted_node n tl)
+let rec sort_nodes (xs : fr_node Prims.list) : fr_node Prims.list=
+  match xs with | [] -> [] | h::tl -> insert_sorted_node h (sort_nodes tl)
+let graph_fuel (g : fr_node Prims.list) : Prims.nat=
+  ((Prims.of_int (4)) * (FStar_List_Tot_Base.length g)) + (Prims.of_int (16))
+let emit_named_nodes (g : fr_node Prims.list)
+  (refids : Prims.string Prims.list) (cl_mode : Prims.bool) :
+  Parser_JSON.json_val Prims.list=
+  let fuel = graph_fuel g in
+  let survivors =
+    FStar_List_Tot_Base.filter
+      (fun n ->
+         ((Prims.op_Negation (is_collapsible g refids n.n_id fuel)) &&
+            (Prims.op_Negation
+               (cl_mode && (is_cl_collapsible g refids n.n_id))))
+           &&
+           ((Prims.uu___is_Cons n.n_types) || (Prims.uu___is_Cons n.n_props)))
+      g in
+  let rewritten =
+    FStar_List_Tot_Base.map (rewrite_node g refids cl_mode fuel) survivors in
+  let ordered = sort_nodes rewritten in
+  FStar_List_Tot_Base.map
+    (fun n -> node_to_json n FStar_Pervasives_Native.None) ordered
+let emit_default_nodes (dm : fr_node Prims.list)
+  (named : named_nm Prims.list) (refids : Prims.string Prims.list)
+  (cl_mode : Prims.bool) : Parser_JSON.json_val Prims.list=
+  let fuel = graph_fuel dm in
+  let survivors =
+    FStar_List_Tot_Base.filter
+      (fun n ->
+         ((Prims.op_Negation (is_collapsible dm refids n.n_id fuel)) &&
+            (Prims.op_Negation
+               (cl_mode && (is_cl_collapsible dm refids n.n_id))))
+           &&
+           (((Prims.uu___is_Cons n.n_types) || (Prims.uu___is_Cons n.n_props))
+              || (is_graph_name named n.n_id))) dm in
+  let rewritten =
+    FStar_List_Tot_Base.map (rewrite_node dm refids cl_mode fuel) survivors in
+  let ordered = sort_nodes rewritten in
+  FStar_List_Tot_Base.map
+    (fun n ->
+       let gj =
+         if is_graph_name named n.n_id
+         then
+           match lookup_graph_map named n.n_id with
+           | FStar_Pervasives_Native.Some gm ->
+               FStar_Pervasives_Native.Some
+                 (emit_named_nodes gm refids cl_mode)
+           | FStar_Pervasives_Native.None -> FStar_Pervasives_Native.Some []
+         else FStar_Pervasives_Native.None in
+       node_to_json n gj) ordered
+let from_rdf (ds : RDF_Graph.rdf_dataset) (opts : from_rdf_options) :
+  Parser_JSON.json_val FStar_Pervasives_Native.option=
+  match build_nodemap opts [] ds.RDF_Graph.ds_default with
+  | FStar_Pervasives_Native.None -> FStar_Pervasives_Native.None
+  | FStar_Pervasives_Native.Some dm0 ->
+      (match build_named opts ds.RDF_Graph.ds_named with
+       | FStar_Pervasives_Native.None -> FStar_Pervasives_Native.None
+       | FStar_Pervasives_Native.Some named ->
+           let dm = add_graph_names dm0 named in
+           let all_maps = dm ::
+             (FStar_List_Tot_Base.map (fun g -> g.gn_map) named) in
+           let refids = maps_refids all_maps in
+           let cl_mode =
+             opts.rdf_direction =
+               (FStar_Pervasives_Native.Some "compound-literal") in
+           FStar_Pervasives_Native.Some
+             (Parser_JSON.JArray (emit_default_nodes dm named refids cl_mode)))
